All those expressions where the incognita appears in the denominator.

$$
\frac{21}{45} = \frac{7 \cdot 3}{5 \cdot 3 \cdot 3} = \frac{7}{15}
$$



#### Example 1

$$\frac{3x + 6}{x^{2} + 4x + 4} = \frac{3(x + 2)}{(x + 2)(x + 2)} = \frac{3}{(x+2)}$$



## Multiplying and Dividing
$$\frac{4}{3} \cdot \frac{2}{5} = \frac{4 \cdot 2}{3 \cdot 5} = \frac{8}{15}$$$$\frac{\frac{4}{5}}{\frac{2}{3}} = \frac{4}{5} \cdot \frac{3}{2} = \frac{12}{10} = \frac{6}{5}$$
#### Example 1

$$ \frac{\frac{x^{2}+x}{x+4}}{\frac{x+1}{x^{2}-16}} = \frac{x^{2}+x}{x+4} \cdot \frac{x^{2}-16}{x+1} $$

Now, multiply, but don't immediately give the result.

$$
\frac{(x^{2} + x)(x^{2} - 16)}{(x+4)(x+1)} $$Now, factor even more

$$\frac{x(x + 1)(x+4)(x-4)}{(x+4)(x+1)} = x(x-4)$$
## Adding and Subtracting

#### Example 1

$$\frac{7}{6} - \frac{4}{15}$$
You must find the LCD (Least Common Denominator)

$$ 6 = 2 \cdot 3$$
$$15 = 3 \cdot 5$$
$$LCD = 2 \cdot 3 \cdot 5 = 30 $$
And now, we proceed dividing the denominator for the LCD, and multiplying the result for the LCD.

$$\frac{35}{30} - \frac{8}{30} = \frac{27}{30}$$

#### Example 2

$$\frac{3}{2x + 2} + \frac{5}{x^{2} - 1}$$
1. Factor the denominator

$$\frac{3}{2(x + 1)} + \frac{5}{(x+1)(x-1)}$$ 
Taking common terms and not common terms with the highest exponent, we can say that

$$LCD = 2(x+1)(x-1)$$

Now, we have to actually put the LCD in the denominators. In the first monomial, we are missing (x-1) in the denominator. Therefore, how do we obtain it?

We divide the entire LCD for the denominator of the first monomial, and we multiply the result for the nominator. Therefore, we will get

$$\frac{3(x-1)}{2(x+1)(x-1)} + \frac{10}{2(x+1)(x-1)}$$
$$\frac{3(x-1) + 10}{2(x+1)(x-1)}$$