
1. Write in standard form
2. Try to factor, if possible (if not, resolve with the quadratic formula)

#### Example 1

$$y^{2} = 18 - 7y \implies y^{2} + 7y - 18 = 0$$

Find the special polynomial.

$$9 - 2 = 7 $$ $$9 \cdot -2 = -18$$

And the expression becomes
$$(y+9)(y-2) = 0$$
Any expression that gives you zero, per la legge dell'annullamento, either the first quantity has to be zero, or the second quantity has to be zero.
Set factors equal to zero.

$$y+9 = 0 \implies y = -9$$
$$y-2=0 \implies y = 2$$ 
#### Example 2

$$ w^{2} = 121 \implies w^{2} - 121 = 0 \implies (w-11)(x+11) = 0)$$
$$w = 11 \lor w == -11$$

#### Example 3

$$x(x+2) = 7 \implies x^{2}+ 2x - 7 = 0$$
There are no numbers for the special polynomial. Therefore, I use the quadratic expression

$$\frac{-b \pm \sqrt{ b^{2} - 4ac }}{2a} \implies \frac{-2 \pm \sqrt{ 4 - 4(1)(-7) }}{2} $$
$$\frac{-2 \pm \sqrt{ 32 }}{2} \implies \frac{-2 \pm(\sqrt{ 16 }\sqrt{ 2 })}{2} \implies \frac{-2 \pm 4\sqrt{ 2 }}{2}$$

Simplify 4 with the denominator and you get

$$x_{1} = \frac{-2}{2} + \frac{4\sqrt{ 2 }}{2} = -1 + 2\sqrt{ 2 }$$
$$x_{2} = \frac{-2}{2} + \frac{4\sqrt{ 2 }}{2} = -1 - 2\sqrt{ 2 }$$